Raw.v
@@ -1,0 +1,311 @@
+(***********************************************************************)
+(*  v      *   The Coq Proof Assistant  /  The Coq Development Team    *)
+(* <O___,, *        INRIA-Rocquencourt  &  LRI-CNRS-Orsay              *)
+(*   \VV/  *************************************************************)
+(*    //   *      This file is distributed under the terms of the      *)
+(*         *       GNU Lesser General Public License Version 2.1       *)
+(***********************************************************************)
+
+(** * Finite map library, "raw" version *)
+
+(** This "raw" interface isn't meant for general use, see rather
+    the [Interface] file for that. The "raw" version has two interests :
+
+    - Internally, as an intermediate step during the implementations
+      [WeakList] [OrdList], [AVL] and [RBT] proposed in this library;
+
+    - For advanced users, access to a "raw" map datatype allows
+      smaller memory footprint during Coq computations (no proof parts)
+      and hence slightly faster operations, at the expense of more
+      complex reasoning when proving properties later.
+
+    Raw means here that among all inhabitant of the type of maps,
+    we'll only consider these fulfilling some adequacy predicate
+    [Ok] (think for instance of lists that are sorted or trees that
+    are binary search trees). All operations here will have [Ok]
+    pre-conditions, and all operations answering new maps will
+    maintain this adequacy.
+
+    A implementation of the usual [Interface.S] can then be obtained
+    by restricting the type of maps, and then wrapping all operations.
+    In functor [Raw2Maps] below, this is done via a record combining
+    a map and a adequacy proof. [Raw2Maps] is used as the final step
+    in [OrdList], [AVL] and [RBT].
+
+    See [Interface] for the documentation of all these operations
+    and extra explanations.
+*)
+
+From Coq Require Export Bool Equalities Orders SetoidList.
+From MMaps Require Export Interface.
+Set Implicit Arguments.
+Unset Strict Implicit.
+
+Definition Cmp {elt:Type}(cmp:elt->elt->bool) e1 e2 := cmp e1 e2 = true.
+
+Module Type WS (K : DecidableType).
+
+  Definition key := K.t.
+  Hint Transparent key.
+
+  Definition eq_key {elt} (p p':key*elt) := K.eq (fst p) (fst p').
+
+  Definition eq_key_elt {elt} (p p':key*elt) :=
+      K.eq (fst p) (fst p') /\ (snd p) = (snd p').
+
+  Parameter t : Type -> Type.
+  (** the abstract type of maps *)
+
+  (** Is a set well-formed or ill-formed ? *)
+
+  Parameter IsOk : forall {elt}, t elt -> Prop.
+  Class Ok {elt}(m:t elt) : Prop := ok : IsOk m.
+
+  (** In order to be able to validate (at least some) particular sets as
+      well-formed, we ask for a boolean function for (semi-)deciding
+      predicate [Ok]. If [Ok] isn't decidable, [isok] may be the
+      always-false function. *)
+  Parameter isok : forall {elt}, t elt -> bool.
+  Parameter isok_Ok : forall {elt} (m:t elt) `(isok m = true), Ok m.
+
+  Section Ops.
+  Parameter empty : forall {elt}, t elt.
+  Variable elt:Type.
+  Parameter is_empty : t elt -> bool.
+  Parameter add : key -> elt -> t elt -> t elt.
+  Parameter find : key -> t elt -> option elt.
+  Parameter remove : key -> t elt -> t elt.
+  Parameter mem : key -> t elt -> bool.
+  Parameter bindings : t elt -> list (key*elt).
+  Parameter cardinal : t elt -> nat.
+  Parameter fold : forall A: Type, (key -> elt -> A -> A) -> t elt -> A -> A.
+  Parameter equal : (elt -> elt -> bool) -> t elt -> t elt -> bool.
+  Variable elt' elt'' : Type.
+  Parameter map : (elt -> elt') -> t elt -> t elt'.
+  Parameter mapi : (key -> elt -> elt') -> t elt -> t elt'.
+  Parameter merge : (key -> option elt -> option elt' -> option elt'') ->
+                      t elt -> t elt' ->  t elt''.
+  End Ops.
+
+  Declare Instance empty_ok {elt} : Ok (@empty elt).
+  Declare Instance add_ok {elt} (m:t elt) x e `(!Ok m) :
+    Ok (add x e m).
+  Declare Instance remove_ok {elt} (m:t elt) x `(!Ok m) :
+    Ok (remove x m).
+  Declare Instance map_ok {elt elt'}(f:elt->elt') m `(!Ok m) :
+    Ok (map f m).
+  Declare Instance mapi_ok {elt elt'}(f:key->elt->elt') m `(!Ok m) :
+    Ok (mapi f m).
+  Declare Instance merge_ok {elt elt' elt''}
+    (f:key -> option elt -> option elt' -> option elt'') m m'
+    `(!Ok m, !Ok m') :
+    Ok (merge f m m').
+
+  Parameter MapsTo : forall {elt}, key -> elt -> t elt -> Prop.
+  Definition In {elt}(k:key)(m: t elt) : Prop := exists e, MapsTo k e m.
+
+  Section Specs.
+  Context {elt elt' elt'' : Type}.
+  Global Declare Instance MapsTo_compat :
+      Proper (K.eq==>Logic.eq==>Logic.eq==>iff) (@MapsTo elt).
+
+  Variable m m' : t elt.
+  Variable x y : key.
+  Variable e : elt.
+  Parameter find_spec : forall `{!Ok m},
+     find x m = Some e <-> MapsTo x e m.
+  Parameter mem_spec : forall `{!Ok m}, mem x m = true <-> In x m.
+  Parameter empty_spec : find x (@empty elt) = None.
+  Parameter is_empty_spec :
+     is_empty m = true <-> forall x, find x m = None.
+  Parameter add_spec1 : forall `{!Ok m}, find x (add x e m) = Some e.
+  Parameter add_spec2 : forall `{!Ok m},
+    ~K.eq x y -> find y (add x e m) = find y m.
+  Parameter remove_spec1 : forall `{!Ok m}, find x (remove x m) = None.
+  Parameter remove_spec2 : forall `{!Ok m},
+    ~K.eq x y -> find y (remove x m) = find y m.
+  Parameter bindings_spec1 :
+    InA eq_key_elt (x,e) (bindings m) <-> MapsTo x e m.
+  Parameter bindings_spec2w : forall `{!Ok m},
+    NoDupA eq_key (bindings m).
+  Parameter cardinal_spec : cardinal m = length (bindings m).
+  Parameter fold_spec :
+    forall {A} (i : A) (f : key -> elt -> A -> A),
+    fold f m i = fold_left (fun a p => f (fst p) (snd p) a) (bindings m) i.
+
+  Definition Equal (m m':t elt) := forall y, find y m = find y m'.
+  Definition Eqdom (m m':t elt) := forall y, In y m <-> In y m'.
+  Definition Equiv (R:elt->elt->Prop) m m' :=
+   Eqdom m m' /\ (forall k e e', MapsTo k e m -> MapsTo k e' m' -> R e e').
+  Definition Equivb (cmp: elt->elt->bool) := Equiv (Cmp cmp).
+
+  Parameter equal_spec :
+   forall (cmp : elt -> elt -> bool)`{!Ok m, !Ok m'},
+    equal cmp m m' = true <-> Equivb cmp m m'.
+
+  Parameter map_spec : forall (f:elt->elt') m x `{!Ok m},
+    find x (map f m) = option_map f (find x m).
+  Parameter mapi_spec : forall (f:key->elt->elt') m x `{!Ok m},
+    exists y:key, K.eq y x /\ find x (mapi f m) = option_map (f y) (find x m).
+
+  Implicit Types f : key->option elt->option elt'->option elt''.
+
+  Parameter merge_spec1 :
+   forall f m m' x `{!Ok m, !Ok m'},
+     In x m \/ In x m' ->
+     exists y:key, K.eq y x /\
+                   find x (merge f m m') = f y (find x m) (find x m').
+
+  Parameter merge_spec2 :
+    forall f m m' x `{!Ok m, !Ok m'},
+      In x (merge f m m') -> In x m \/ In x m'.
+
+  End Specs.
+End WS.
+
+(** ** Raw Maps on ordered keys. *)
+
+Module Type S (K : OrderedType).
+  Include WS K.
+
+  Definition lt_key {elt} (p p':key*elt) := K.lt (fst p) (fst p').
+
+  Parameter bindings_spec2 :
+    forall {elt}(m : t elt)`{!Ok m}, sort lt_key (bindings m).
+End S.
+
+Module WRaw2Maps (K : DecidableType) (M : WS K) <: Interface.WS K.
+
+ Import M.
+
+ (** We avoid creating induction principles for the Record *)
+ Local Unset Elimination Schemes.
+
+ Record t_ (elt:Type) := Mkt {this :> M.t elt; is_ok : Ok this}.
+ Definition t := t_.
+ Definition key := K.t.
+
+ Hint Unfold t.
+ Existing Instance is_ok.
+ Local Arguments Mkt {elt} this {is_ok}.
+
+ Section Elt.
+ Context {elt elt' elt'': Type}.
+
+ Implicit Types m : t elt.
+ Implicit Types x y : key.
+ Implicit Types e : elt.
+
+ Definition empty : t elt := Mkt (@empty elt).
+ Definition is_empty m : bool := is_empty m.
+ Definition add x e m : t elt := Mkt (add x e m).
+ Definition remove x m : t elt := Mkt (remove x m).
+ Definition mem x m : bool := mem x m.
+ Definition find x m : option elt := find x m.
+ Definition map f m : t elt' := Mkt (map f m).
+ Definition mapi (f:key->elt->elt') m : t elt' := Mkt (mapi f m).
+ Definition merge f m (m':t elt') : t elt'' := Mkt (merge f m m').
+ Definition bindings m : list (key*elt) := bindings m.
+ Definition cardinal m := cardinal m.
+ Definition fold {A} (f:key->elt->A->A) m i := fold f m i.
+ Definition equal cmp m m' : bool := equal cmp m m'.
+
+ Definition MapsTo x e m : Prop := MapsTo x e m.
+ Definition In x m : Prop := In x m.
+
+ Definition eq_key {elt} (p p':key*elt) := K.eq (fst p) (fst p').
+
+ Definition eq_key_elt {elt} (p p':key*elt) :=
+  K.eq (fst p) (fst p') /\ (snd p) = (snd p').
+
+ Instance MapsTo_compat :
+   Proper (K.eq==>Logic.eq==>Logic.eq==>iff) MapsTo.
+ Proof.
+  intros k k' Hk e e' <- m m' <-. unfold MapsTo; simpl. now rewrite Hk.
+ Qed.
+
+ Lemma find_spec m x e : find x m = Some e <-> MapsTo x e m.
+ Proof. apply find_spec, is_ok. Qed.
+
+ Lemma mem_spec m x : mem x m = true <-> In x m.
+ Proof. apply mem_spec, is_ok. Qed.
+
+ Lemma empty_spec x : find x empty = None.
+ Proof. apply empty_spec. Qed.
+
+ Lemma is_empty_spec m : is_empty m = true <-> forall x, find x m = None.
+ Proof. apply is_empty_spec. Qed.
+
+ Lemma add_spec1 m x e : find x (add x e m) = Some e.
+ Proof. apply add_spec1, is_ok. Qed.
+ Lemma add_spec2 m x y e : ~ K.eq x y -> find y (add x e m) = find y m.
+ Proof. apply add_spec2, is_ok. Qed.
+
+ Lemma remove_spec1 m x : find x (remove x m) = None.
+ Proof. apply remove_spec1, is_ok. Qed.
+ Lemma remove_spec2 m x y : ~K.eq x y -> find y (remove x m) = find y m.
+ Proof. apply remove_spec2, is_ok. Qed.
+
+ Lemma bindings_spec1 m x e :
+   InA eq_key_elt (x,e) (bindings m) <-> MapsTo x e m.
+ Proof. apply bindings_spec1. Qed.
+
+ Lemma bindings_spec2w m : NoDupA eq_key (bindings m).
+ Proof. apply bindings_spec2w, is_ok. Qed.
+
+ Lemma fold_spec m {A} (i : A) (f : key -> elt -> A -> A) :
+   fold f m i = fold_left (fun a p => f (fst p) (snd p) a) (bindings m) i.
+ Proof. apply fold_spec. Qed.
+
+ Lemma cardinal_spec m : cardinal m = length (bindings m).
+ Proof. apply cardinal_spec. Qed.
+
+ Definition Equal m m' := forall y, find y m = find y m'.
+ Definition Eqdom (m m':t elt) := forall y, In y m <-> In y m'.
+ Definition Equiv (R:elt->elt->Prop) m m' :=
+  Eqdom m m' /\ (forall k e e', MapsTo k e m -> MapsTo k e' m' -> R e e').
+ Definition Equivb cmp := Equiv (Cmp cmp).
+
+ Lemma Equivb_Equivb cmp m m' :
+  Equivb cmp m m' <-> M.Equivb cmp m m'.
+ Proof.
+ unfold Equivb, Equiv, M.Equivb, M.Equiv. intuition.
+ Qed.
+
+ Lemma equal_spec m m' cmp :
+   equal cmp m m' = true <-> Equivb cmp m m'.
+ Proof. rewrite Equivb_Equivb. apply equal_spec; apply is_ok. Qed.
+
+ End Elt.
+
+ Lemma map_spec {elt elt'} (f:elt->elt') m x :
+   find x (map f m) = option_map f (find x m).
+ Proof. apply map_spec, is_ok. Qed.
+
+ Lemma mapi_spec {elt elt'} (f:key->elt->elt') m x :
+   exists y:key, K.eq y x /\ find x (mapi f m) = option_map (f y) (find x m).
+ Proof. apply mapi_spec, is_ok. Qed.
+
+ Lemma merge_spec1 {elt elt' elt''}
+       (f:key->option elt->option elt'->option elt'') m m' x :
+   In x m \/ In x m' ->
+   exists y:key, K.eq y x /\
+                 find x (merge f m m') = f y (find x m) (find x m').
+ Proof. apply merge_spec1; apply is_ok. Qed.
+
+ Lemma merge_spec2 {elt elt' elt''}
+       (f:key -> option elt->option elt'->option elt'') m m' x :
+   In x (merge f m m') -> In x m \/ In x m'.
+ Proof. apply merge_spec2; apply is_ok. Qed.
+
+End WRaw2Maps.
+
+Module Raw2Maps (K : OrderedType) (M : S K) <: Interface.S K.
+ Include WRaw2Maps K M.
+
+ Definition lt_key {elt} (p p':key*elt) := K.lt (fst p) (fst p').
+
+ Lemma bindings_spec2 {elt}(m : t elt) : sort lt_key (bindings m).
+ Proof. apply M.bindings_spec2. Qed.
+
+End Raw2Maps.
